\input{../utils/preamble}
\createdgmtitle{10}

\usepackage{tikz}

\usetikzlibrary{arrows,shapes,positioning,shadows,trees}
%--------------------------------------------------------------------------------
\begin{document}
%--------------------------------------------------------------------------------
\begin{frame}[noframenumbering,plain]
%\thispagestyle{empty}
\titlepage
\end{frame}
%=======
\begin{frame}{Recap of previous lecture}
	Let take some pretrained image classification model to get the conditional label distribution $p(y | \bx)$ (e.g. ImageNet classifier).
	\begin{block}{Evaluation of likelihood-free models}
		\begin{itemize}
			\item Sharpness $\Rightarrow$ low $H(y | \bx) = - \sum_{y} \int_{\bx} p(y, \bx) \log p(y | \bx) d\bx$.
			\item Diversity $\Rightarrow$ high $H(y)  = - \sum_{y} p(y) \log p(y)$.
		\end{itemize}
	\end{block}
	\vspace{-0.3cm}
	\begin{block}{Inception Score}
		\vspace{-0.2cm}
		\[
			IS = \exp(H(y) - H(y | \bx)) = \exp \left( \bbE_{\bx} KL(p(y | \bx) || p(y)) \right)
		\]
		\vspace{-0.5cm}
	\end{block}
	\begin{block}{Frechet Inception Distance}
		\vspace{-0.3cm}
		\[
			D^2 (\pi, p) = \| \mathbf{m}_{\pi} - \mathbf{m}_{p}\|_2^2 + \text{Tr} \left( \bSigma_{\pi} + \bSigma_p - 2 \sqrt{\bSigma_{\pi} \bSigma_p} \right).
		\]
		\vspace{-0.5cm}
	\end{block}
	FID is related to moment matching.
	
	\myfootnote{\href{https://arxiv.org/abs/1606.03498}{Salimans T. et al. Improved Techniques for Training GANs, 2016} \\
	\href{https://arxiv.org/abs/1706.08500}{Heusel M. et al. GANs Trained by a Two Time-Scale Update Rule Converge to a Local Nash Equilibrium, 2017} }
\end{frame}
%=======
\begin{frame}{Recap of previous lecture}
		\begin{itemize}
			\item $\cS_{\pi} = \{\bx_i\}_{i=1}^{n} \sim \pi(\bx)$ -- real samples;
			\item $\cS_{p} = \{\bx_i\}_{i=1}^{n} \sim p(\bx | \btheta)$ -- generated samples.
		\end{itemize}
		Embed samples using pretrained classifier network (as previously):
		\[
			\cG_{\pi} = \{\mathbf{g}_i\}_{i=1}^n, \quad \cG_{p} = \{\mathbf{g}_i\}_{i=1}^n.
		\]
		Define binary function:
		\[
			f(\mathbf{g}, \cG) = 
			\begin{cases}
				1, \text{if exists } \mathbf{g}' \in \cG: \| \mathbf{g}  - \mathbf{g}'\|_2 \leq \| \mathbf{g}' - \text{NN}_k(\mathbf{g}', \cG)\|_2; \\
				0, \text{otherwise.}
			\end{cases}
		\]
		\[
			\text{Precision} (\cG_{\pi}, \cG_{p}) = \frac{1}{n} \sum_{\mathbf{g} \in \cG_{p}} f(\mathbf{g}, \cG_{\pi}); \quad \text{Recall} (\cG_{\pi}, \cG_{p}) = \frac{1}{n} \sum_{\mathbf{g} \in \cG_{\pi}} f(\mathbf{g}, \cG_{p}).
		\]
		\vspace{-0.4cm}
		\begin{figure}
			\includegraphics[width=0.7\linewidth]{figs/pr_k_nearest}
		\end{figure}
		\myfootnotewithlink{https://arxiv.org/abs/1904.06991}{Kynkäänniemi T. et al. Improved precision and recall metric for assessing generative models, 2019}
\end{frame}
%=======
\begin{frame}{Outline}
	\tableofcontents
\end{frame}
%=======
\begin{frame}{Generative models zoo}
	\begin{tikzpicture}[
		basic/.style  = {draw, text width=2cm, drop shadow, rectangle},
		root/.style   = {basic, rounded corners=2pt, thin, text height=1.1em, text width=7em, align=center, fill=blue!40},
		level 1/.style={sibling distance=55mm},
		level 2/.style = {basic, rounded corners=6pt, thin, align=center, fill=blue!20, text height=1.1em, text width=9em, sibling distance=38mm},
		level 3/.style = {basic, rounded corners=6pt, thin,align=center, fill=blue!20, text width=8.5em},
		level 4/.style = {basic, thin, align=left, fill=pink!30, text width=7em},
		level 5/.style = {basic, thin, align=left, fill=pink!90, text width=7em},
		edge from parent/.style={->,draw},
		>=latex]
		
		% root of the the initial tree, level 1
		\node[root] {\Large Generative models}
		% The first level, as children of the initial tree
		child {node[level 2] (c1) {Likelihood-based}
			child {node[level 3] (c11) {Tractable density}}
			child {node[level 3] (c12) {Approximate density}}
		}
		child {node[level 2] (c2) {Implicit density}};
		
		% The second level, relatively positioned nodes
		\begin{scope}[every node/.style={level 4}]
			\node [below of = c11, yshift=-5pt, xshift=10pt] (c111) {Autoregressive models};
			\node [below of = c111, yshift=-5pt] (c112) {Normalizing Flows};
			\node [below of = c12, xshift=10pt] (c121) {VAEs};
			
			\node [below of = c2, xshift=10pt] (c21) {GANs};
		\end{scope}
		
		% The second level, relatively positioned nodes
		\begin{scope}[every node/.style={level 5}]
			\node [below of = c121] (c122) {\textbf{Diffusion \\ models}};
		\end{scope}
		
		% lines from each level 1 node to every one of its "children"
		\foreach \value in {1,2}
		\draw[->] (c11.194) |- (c11\value.west);
		
		\foreach \value in {1,2}
		\draw[->] (c12.194) |- (c12\value.west);
		
		\draw[->] (c2.194) |- (c21.west);
		
	\end{tikzpicture}
\end{frame}
%=======
\section{Gaussian diffusion process}
%=======
\subsection{Forward gaussian diffusion process}
%=======
\begin{frame}{Forward gaussian diffusion process}
	Let $\bx_0 = \bx \sim \pi(\bx)$, $\beta_t \in (0, 1)$. Define the Markov chain
	\[
		\bx_t = \sqrt{1 - \beta_t} \cdot \bx_{t - 1} + \sqrt{\beta_t} \cdot \bepsilon, \quad \text{where }\bepsilon \sim \cN(0, \bI);
	\]
	\[
		q(\bx_t | \bx_{t-1}) = \cN(\bx_t | \sqrt{1 - \beta_t} \cdot \bx_{t-1}, \beta_t \cdot \bI).
	\]
	\vspace{-0.5cm}
	\begin{block}{Statement 1}
		Let denote $\alpha_t = 1 - \beta_t$ and $\bar{\alpha}_t = \prod_{s=1}^t \alpha_s$. Then
		\vspace{-0.2cm}
		\begin{multline*}
			\bx_t = \sqrt{\alpha_t} {\color{teal}\bx_{t-1}} + \sqrt{1 - \alpha_t} \boldsymbol{\epsilon}_t = \\
			= \sqrt{\alpha_t} ({\color{teal} \sqrt{\alpha_{t-1}} \bx_{t-2} + \sqrt{1 - \alpha_{t-1}} \boldsymbol{\epsilon}_{t-1}}) + \sqrt{1 - \alpha_t} \boldsymbol{\epsilon}_t = \\
			= \sqrt{\alpha_t \alpha_{t-1}} \bx_{t-2} + ( \sqrt{\alpha_t (1 - \alpha_{t-1})}  \boldsymbol{\epsilon}_{t-1} + \sqrt{1 - \alpha_t} \boldsymbol{\epsilon}_t) = \\
			= \sqrt{\bar{\alpha}_t} \cdot \bx_{0} + \sqrt{1 - \bar{\alpha}_t} \cdot \bepsilon, \quad \text{where } \bepsilon \sim \cN(0, \bI).
		\end{multline*}
		\vspace{-0.4cm}
		\[
			q(\bx_t | \bx_0) = \cN(\bx_t | \sqrt{\bar{\alpha}_t} \cdot \bx_0, (1 - \bar{\alpha}_t) \cdot \bI).
		\]
		We could sample from any timestamp using only $\bx_0$!
	\end{block}
	\myfootnotewithlink{http://proceedings.mlr.press/v37/sohl-dickstein15.pdf}{Sohl-Dickstein J. Deep Unsupervised Learning using Nonequilibrium Thermodynamics, 2015}
 \end{frame}
%=======
\begin{frame}{Forward gaussian diffusion process}
	\vspace{-0.5cm}
	\begin{align*}
		q(\bx_t | \bx_{t-1}) &= \cN(\bx_t | \sqrt{1 - \beta_t} \cdot \bx_{t-1}, \beta_t \cdot \bI); \\
		q(\bx_t | \bx_0) &= \cN(\bx_t | \sqrt{\bar{\alpha}_t} \cdot \bx_0, (1 - \bar{\alpha}_t) \cdot \bI).
	\end{align*}
	At each step we
	\begin{itemize}
		\item scale magnitude of the signal at rate $\sqrt{1 - \beta_t}$;
		\item add noise with variance $\beta_t$.
	\end{itemize}
	\begin{block}{Statement 2}
		Applying the Markov chain to samples from any $\pi(\bx)$ we will get $\bx_{\infty} \sim p_{\infty}(\bx) = \cN(0, 1)$. Here $p_{\infty}(\bx)$ is a \textbf{stationary} and \textbf{limiting} distribution:
		\vspace{-0.2cm}
		\[
			p_{\infty}(\bx) = \int q(\bx | \bx') p_{\infty}(\bx') d \bx'. 
		\]
		\[
			p_{\infty}(\bx) = \int q(\bx_{\infty} | \bx_0) \pi(\bx_0) d\bx_0 \approx \cN(0, \bI) \int \pi(\bx_0) d\bx_0 = \cN(0, \bI)
		\]
		\vspace{-0.8cm}
	\end{block}
	\myfootnotewithlink{http://proceedings.mlr.press/v37/sohl-dickstein15.pdf}{Sohl-Dickstein J. Deep Unsupervised Learning using Nonequilibrium Thermodynamics, 2015}
 \end{frame}
%=======
\begin{frame}{Forward gaussian diffusion process}
	\textbf{Diffusion} refers to the flow of particles from high-density regions towards low-density regions.
	\vspace{-0.2cm}
	\begin{figure}
		\includegraphics[width=0.5\linewidth]{figs/diffusion_over_time}
	\end{figure}
	\vspace{-0.6cm}
	\begin{enumerate}
		\item $\bx_0 = \bx \sim \pi(\bx)$;
		\item $\bx_t = \sqrt{1 - \beta_t} \cdot \bx_{t - 1} + \sqrt{\beta_t} \cdot \bepsilon$, where $\bepsilon \sim \cN(0, 1)$, $t \geq 1$;
		\item $\bx_T \sim p_{\infty}(\bx) = \cN(0, 1)$, where $T >> 1$.
	\end{enumerate}
	If we are able to invert this process, we will get the way to sample $\bx \sim \pi(\bx)$ using noise samples $p_{\infty}(\bx) = \cN(0, \mathbf{I})$. \\ 
	Now our goal is to revert this process.
	\myfootnotewithlink{https://ayandas.me/blog-tut/2021/12/04/diffusion-prob-models.html}{Das A. An introduction to Diffusion Probabilistic Models, blog post, 2021}
\end{frame}
%=======
\subsection{Reverse gaussian diffusion process}
%=======
\begin{frame}{Reverse gaussian diffusion process}
	\begin{figure}
		\includegraphics[width=0.8\linewidth]{figs/DDPM}
	\end{figure}
	\vspace{-0.5cm}
	\begin{block}{Forward process}
		\vspace{-0.3cm}
		\[
			q(\bx_t | \bx_{t-1}) = \cN(\bx_t | \sqrt{1 - \beta_t} \cdot \bx_{t-1}, \beta_t \cdot \bI).
		\]
		\vspace{-0.5cm}
	\end{block}
	\begin{block}{Reverse process}
		\vspace{-0.3cm}
		\[
			q(\bx_{t-1}|\bx_{t}) = \frac{q(\bx_{t}|\bx_{t-1}) {\color{violet}q(\bx_{t-1})}}{{\color{violet}q(\bx_{t})}} \approx p(\bx_{t - 1} | \bx_t, \btheta)
		\]
		\vspace{-0.3cm}
		\begin{itemize}
			\item ${\color{violet}q(\bx_{t-1})}$, ${\color{violet}q(\bx_{t})}$ are intractable.
			\item If $\beta_t$ is small enough, $q(\bx_{t-1}|\bx_{t})$ will be Gaussian (Feller, 1949).
		\end{itemize}
	\end{block}
	\myfootnotewithlink{}{Feller W. On the theory of stochastic processes, with particular reference to applications, 1949}
	\end{frame}
%=======
\begin{frame}{Reverse gaussian diffusion process}
		\vspace{-0.4cm}
		\begin{align*}
			q(\bx_{t-1}|\bx_{t}) &= \frac{q(\bx_{t}|\bx_{t-1}) {\color{violet}q(\bx_{t-1})}}{{\color{violet}q(\bx_{t})}} \\
			q(\bx_{t-1}|\bx_{t}, {\color{olive}\bx_0}) &= \frac{q(\bx_{t}|\bx_{t-1}, {\color{olive}\bx_0}) q(\bx_{t-1} | {\color{olive}\bx_0}) }{q(\bx_{t}| {\color{olive}\bx_0})} = \cN(\tilde{\bmu}_t(\bx_t, \bx_0), \tilde{\beta}_t \bI)
		\end{align*}
		\vspace{-0.2cm}
		\begin{itemize}
			\item ${\color{violet}q(\bx_{t-1})}$, ${\color{violet}q(\bx_{t})}$ are intractable.
			\item If $\beta_t$ is small enough, $q(\bx_{t-1}|\bx_{t})$ will be Gaussian (Feller, 1949).
		\end{itemize}
	\vspace{-0.2cm}
	\begin{figure}
		\includegraphics[width=0.7\linewidth]{figs/inverse_distr_1d}
	\end{figure}
	\myfootnotewithlink{https://arxiv.org/abs/2112.07804}{Xiao Z., Kreis K., Vahdat A. Tackling the generative learning trilemma with denoising diffusion GANs, 2021}
	\end{frame} 
%=======
\begin{frame}{Reverse gaussian diffusion process}
	\vspace{-0.3cm} 
	\begin{figure}
		\includegraphics[width=0.8\linewidth]{figs/DDPM}
	\end{figure}
	\vspace{-0.3cm} 
	Let define the reverse process
	\vspace{-0.2cm}
	\[
		q(\bx_{t-1}|\bx_{t}) \approx p(\bx_{t - 1} | \bx_t, \btheta) = \cN \bigl(\bx_{t - 1} | \bmu_{\btheta}(\bx_t, t), \bsigma_{\btheta}^2(\bx_t, t)\bigr)
	\]
	\vspace{-0.7cm}
	\begin{minipage}{0.5\linewidth}
		\begin{block}{Forward process}
			\begin{enumerate}
				\item $\bx_0 = \bx \sim \pi(\bx)$;
				\item $\bx_t = \sqrt{1 - \beta_t} \cdot \bx_{t - 1} + \sqrt{\beta_t} \cdot \bepsilon$, where $\bepsilon \sim \cN(0, \bI)$, $t \geq 1$;
				\item $\bx_T \sim p_{\infty}(\bx) = \cN(0, \bI)$.
			\end{enumerate}
		\end{block}
	\end{minipage}%
	\begin{minipage}{0.5\linewidth}
		\begin{block}{Reverse process}
			\begin{enumerate}
				\item $\bx_T \sim p_{\infty}(\bx) = \cN(0, \bI)$;
				\item $\bx_{t - 1} = \bsigma_{\btheta}(\bx_t, t) \cdot \bepsilon + \bmu_{\btheta}(\bx_t, t)$;
				\item $\bx_0 = \bx \sim \pi(\bx)$;
			\end{enumerate}
		\end{block}
	\end{minipage}
	\textbf{Note:} The forward process does not have any learnable parameters!
	\myfootnotewithlink{https://lilianweng.github.io/posts/2021-07-11-diffusion-models/}{Weng L. What are Diffusion Models?, blog post, 2021}
\end{frame}
%=======
\section{Gaussian diffusion model as VAE}
%=======
\begin{frame}{Gaussian diffusion model as VAE}
	\vspace{-0.2cm}
	\begin{figure}
		\includegraphics[width=0.65\linewidth]{figs/diffusion_pgm}
	\end{figure}
	\begin{itemize}
		\item Let treat $\bz = (\bx_1, \dots, \bx_T)$ as a latent variable (\textbf{note:} each $\bx_t$ has the same size).
		\item Variational posterior distribution (\textbf{note:} there is no learnable parameters)
		\vspace{-0.4cm}
		\[
			q(\bz | \bx) = q(\bx_1, \dots, \bx_T | \bx_0) = \prod_{t = 1}^T q(\bx_t | \bx_{t - 1}).
		\]
		\vspace{-0.5cm}
		\item Probabilistic model
		\vspace{-0.2cm}
		\[
			p(\bx, \bz | \btheta) = p(\bx | \bz, \btheta) p(\bz | \btheta)
		\]
		\item Generative distribution and prior
		\vspace{-0.3cm}
		\[
			p(\bx | \bz, \btheta) = p(\bx_0 | \bx_1, \btheta); \quad 
			p(\bz | \btheta) = \prod_{t=2}^T p(\bx_{t - 1} | \bx_t, \btheta)  \cdot p(\bx_T)
		\]
	\end{itemize}
	\myfootnotewithlink{https://ayandas.me/blog-tut/2021/12/04/diffusion-prob-models.html}{Das A. An introduction to Diffusion Probabilistic Models, blog post, 2021}
\end{frame}
%=======
\begin{frame}{ELBO for gaussian diffusion model}
	\begin{block}{Standard ELBO}
		\vspace{-0.4cm}
		\[
			\log p(\bx | \btheta) \geq \bbE_{q({\color{teal}\bz} | \bx)} \log \frac{p(\bx, {\color{teal}\bz} | \btheta)}{q({\color{teal}\bz} | \bx)} = \cL(q, \btheta) \rightarrow \max_{q, \btheta}
		\]
		\vspace{-0.5cm}
	\end{block}
	\begin{block}{Derivation}
		\vspace{-0.5cm}
		{\small
		\begin{align*}
			\cL(q, \btheta) &= \bbE_{q({\color{teal}\bx_{1:T}} | \bx_0)} \log \frac{p(\bx_0, {\color{teal}\bx_{1:T}} | \btheta)}{q({\color{teal}\bx_{1:T}} | \bx_0)} \\
			& = \bbE_{q(\bx_{1:T} | \bx_0)} \log \frac{p(\bx_T) \prod_{t=1}^T p(\bx_{t-1} | \bx_t, \btheta) }{\prod_{t=1}^T q(\bx_t | \bx_{t-1})}  \\ 
			& = \bbE_{q(\bx_{1:T} | \bx_0)} \log \frac{p(\bx_T) p(\bx_0 | \bx_1, \btheta) \prod_{t=2}^T p(\bx_{t-1} | \bx_t, \btheta) }{q(\bx_1 | \bx_0)\prod_{t=2}^T {\color{teal}q(\bx_t | \bx_{t-1})}}  \\ 
			& = \bbE_{q(\bx_{1:T} | \bx_0)} \log \frac{p(\bx_T) p(\bx_0 | \bx_1, \btheta) \prod_{t=2}^T p(\bx_{t-1} | \bx_t, \btheta) }{q(\bx_1 | \bx_0)\prod_{t=2}^T q(\bx_t | \bx_{t-1}, {\color{olive}\bx_0})} 
		\end{align*}
		}
		\[
			q(\bx_{t-1}|\bx_{t}, {\color{olive}\bx_0}) = \frac{q(\bx_{t}|\bx_{t-1}, {\color{olive}\bx_0}) q(\bx_{t-1} | {\color{olive}\bx_0}) }{q(\bx_{t}| {\color{olive}\bx_0})} = \cN(\tilde{\bmu}_t(\bx_t, \bx_0), \tilde{\beta}_t \bI)
		\]
	\end{block}
	
	\myfootnotewithlink{https://arxiv.org/abs/2006.11239}{Ho J. Denoising Diffusion Probabilistic Models, 2020}
\end{frame}
%=======
\begin{frame}{ELBO for gaussian diffusion model}
	\begin{block}{Derivation (continued)}
		\vspace{-0.7cm}
		{\small
		\begin{multline*}
			\cL(q, \btheta) = \bbE_{q(\bx_{1:T} | \bx_0)} \log \frac{p(\bx_T) p(\bx_0 | \bx_1, \btheta) \prod_{t=2}^T p(\bx_{t-1} | \bx_t, \btheta) }{q(\bx_1 | \bx_0)\prod_{t=2}^T q(\bx_t | \bx_{t-1}, {\color{olive}\bx_0})}  = \\ 
			= \bbE_{q(\bx_{1:T} | \bx_0)} \log \frac{p(\bx_T) p(\bx_0 | \bx_1, \btheta) \prod_{t=2}^T p(\bx_{t-1} | \bx_t, \btheta) }{{\color{violet}q(\bx_1 | \bx_0)}\prod_{t=2}^T \frac{q(\bx_{t-1}|\bx_t, \bx_0) {\color{violet}q(\bx_{t} | \bx_0)}}{{\color{violet}q(\bx_{t-1}| \bx_0)}}}  = \\
			= \bbE_{q(\bx_{1:T} | \bx_0)} \log \frac{{\color{violet}p(\bx_T)} {\color{olive}p(\bx_0 | \bx_1, \btheta)} \prod_{t=2}^T p(\bx_{t-1} | \bx_t, \btheta) }{{\color{violet}q(\bx_T | \bx_0)}\prod_{t=2}^T q(\bx_{t-1}|\bx_t, \bx_0)}  = \\
			= \bbE_{{\color{teal}q(\bx_{1:T} | \bx_0)}} \biggl[ \log {\color{olive}p(\bx_0 | \bx_1, \btheta)} + \log {\color{violet}\frac{p(\bx_T)}{q(\bx_T | \bx_0)}} + \sum_{t=2}^T \log \left( \frac{p(\bx_{t-1} | \bx_t, \btheta)}{q(\bx_{t-1}|\bx_{t}, \bx_0)}\right) \biggr] = \\
			 = \bbE_{{\color{teal}q(\bx_1 | \bx_0)}} \log p(\bx_0 | \bx_1, \btheta) + \bbE_{{\color{teal}q(\bx_T | \bx_0)}} \log \frac{p(\bx_T)}{q(\bx_T | \bx_0)} + \\
			  + \sum_{t=2}^T \bbE_{{\color{teal}q(\bx_{t-1}, \bx_t | \bx_0)}} \log \left( \frac{p(\bx_{t-1} | \bx_t, \btheta)}{q(\bx_{t-1}|\bx_{t}, \bx_0)}\right) 
		\end{multline*}
		}
		\vspace{-0.3cm}
	\end{block}
	\myfootnotewithlink{https://arxiv.org/abs/2006.11239}{Ho J. Denoising Diffusion Probabilistic Models, 2020}
\end{frame}
%=======
\begin{frame}{ELBO for gaussian diffusion model}
		\vspace{-0.5cm}
		\begin{multline*}
			\cL(q, \btheta) = \bbE_{q(\bx_1 | \bx_0)} \log p(\bx_0 | \bx_1, \btheta) + \bbE_{q(\bx_T | \bx_0)} \log \frac{p(\bx_T)}{q(\bx_T | \bx_0)} + \\
			  + \sum_{t=2}^T \bbE_{q(\bx_{t-1}, \bx_t | \bx_0)} \log \left( \frac{p(\bx_{t-1} | \bx_t, \btheta)}{q(\bx_{t-1}|\bx_{t}, \bx_0)}\right) =
			  \\ =  {\color{olive}\bbE_{q(\bx_1 | \bx_0)} \log p(\bx_0 | \bx_1, \btheta)} - {\color{violet}KL\bigl(q(\bx_T | \bx_0) || p(\bx_T)\bigr)} - \\
			- \sum_{t=2}^T \underbrace{ \bbE_{q(\bx_t | \bx_0)} KL \bigl(q(\bx_{t-1} | \bx_t, \bx_0) || p(\bx_{t - 1} | \bx_t, \btheta )\bigr)}_{\cL_t}
		\end{multline*}
		\vspace{-0.5cm}
	\begin{itemize}
		\item {\color{olive}First term} is a decoder distribution
		\[
			\log p(\bx_0 | \bx_1, \btheta) = \log \cN \bigl(\bx_0 | \bmu_{\btheta}(\bx_1, t), \bsigma_{\btheta}^2(\bx_1, t)\bigr).
		\] 
		\item {\color{violet}Second term} is constant ($p(\bx_T)$ is a standard Normal, $q(\bx_T | \bx_0)$ is a non-parametrical Normal).
	\end{itemize}
	\myfootnotewithlink{https://arxiv.org/abs/2006.11239}{Ho J. Denoising Diffusion Probabilistic Models, 2020}
\end{frame}
%=======
\begin{frame}{ELBO for gaussian diffusion model}
	\vspace{-0.5cm}
	\begin{multline*}
		\cL(q, \btheta) =  {\color{olive}\bbE_{q(\bx_1 | \bx_0)} \log p(\bx_0 | \bx_1, \btheta)} - {\color{violet}KL\bigl(q(\bx_T | \bx_0) || p(\bx_T)\bigr)} - \\
		- \sum_{t=2}^T \underbrace{ \bbE_{q(\bx_t | \bx_0)} KL \bigl(q(\bx_{t-1} | \bx_t, \bx_0) || p(\bx_{t - 1} | \bx_t, \btheta )\bigr)}_{\cL_t}
	\end{multline*}
	$q(\bx_{t-1} | \bx_t, \bx_0)$ defines how to denoise a noisy image $\bx_t$ with access to what the final, completely denoised image $\bx_0$ should be.
	
	\begin{figure}
		\includegraphics[width=0.85\linewidth]{figs/diffusion_objective}
	\end{figure}

	\myfootnotewithlink{https://arxiv.org/abs/2208.11970}{Luo C. Understanding Diffusion Models: A Unified Perspective, 2022}
\end{frame}
%=======
\begin{frame}{Summary}
	\begin{itemize}
		\item Gaussian diffusion process is a Markov chain that injects special form of Gaussian noise to the samples.
		\vfill
		\item Reverse process allows to sample from the real distribution $\pi(\bx)$ using samples from noise.
		\vfill
		\item Diffusion model is a VAE model which reverts gaussian diffusion process using variational inference.
		\vfill
		\item ELBO of DDPM could be represented as a sum of KL terms.
	\end{itemize}
\end{frame}
\end{document} 